Ex1

teaching/taltech2018/ex/ex1/Sum.fst
@@ -4,22 +4,19 @@ open FStar.Mul
 
 (* 
 
-  Exercise 1: 
-   
-     1.1 Define a recursive total function `sum` that sums up natural numbers from 1 to n.
-         (That is, replace the 1st `admit ()` with an appropriate recursive definition.)
+  In this exercise you will practice defining recursive functions and doing proofs about them
+     
+  Task 1: Define a recursive total function `sum` that sums up natural numbers from 1 to n.
+          That is, replace the 1st `admit ()` with an appropriate recursive definition.
 
-     1.2 Prove that `sum` is equal to the nth triangual number (as computed by `triangular`).
-         (That is, replace the 2nd `admit ()` with a proof of `sum n = triangular n`.)
+  Task 2: Prove that `sum` is equal to the nth triangual number (as computed by the function `triangular`).
+          That is, replace the 2nd `admit ()` with a proof of `sum n = triangular n`.
          
 *)
 
 
-let rec sum (n:nat) : Tot nat = 
-  admit ()
+let rec sum (n:nat) : Tot nat = admit ()
 
-let nth_triangular (n:nat) : GTot nat = 
-  ((n+1) * n) / 2
+let nth_triangular (n:nat) : GTot nat = ((n+1) * n) / 2
 
-let rec sum_correct (n:nat) : Lemma (sum n = nth_triangular n) =
-  admit ()
+let rec sum_correct (n:nat) : Lemma (sum n = nth_triangular n) = admit ()
