teaching/taltech2018/sols_hidden/ex2/Stack.fsti
@@ -1,15 +1,12 @@
 module Stack
 
-// BEGIN: stack_types
-val stack : Type0  (* type of stacks *)
+val stack : Type0
 val empty : stack
 val is_empty : stack -> GTot bool
 val push : int -> stack -> stack
 val pop : stack -> option stack
 val top : stack -> option int
-// END: stack_types
 
-// BEGIN: stack_lemmas
 val lemma_empty_is_empty : unit -> Lemma (is_empty (empty))
 
 val lemma_push_is_empty : s:stack -> i:int ->
@@ -22,11 +19,12 @@ val lemma_is_empty_pop_some : s:stack{~(is_empty s)} ->
   Lemma (Some? (pop s)) [SMTPat (pop s)]
 
 val lemma_push_top : s:stack -> i:int -> 
-  Lemma (Some? (top (push i s)) /\ Some?.v (top (push i s)) = i) [SMTPat (top (push i s))]
+  Lemma (Some? (top (push i s)) /\ Some?.v (top (push i s)) = i) 
+  [SMTPat (top (push i s))]
                                                   
 val lemma_push_pop : s:stack -> i:int -> 
-  Lemma (Some? (pop (push i s)) /\ Some?.v (pop (push i s)) == s) [SMTPat (pop (push i s))]
+  Lemma (Some? (pop (push i s)) /\ Some?.v (pop (push i s)) == s) 
+  [SMTPat (pop (push i s))]
 
 val lemma_top_pop_push : s:stack{~(is_empty s)} ->  
   Lemma (push (Some?.v (top s)) (Some?.v (pop s)) == s)
-// END: stack_lemmas
